case_study/MinimalCaps/Model.v
@@ -604,19 +604,58 @@ Module MinCapsIrisInstanceWithContracts.
       rewrite fixpoint_interp1_eq; auto.
     Qed.
 
+    Lemma correctPC_not_E_sound :
+      ValidLemma lemma_correctPC_not_E.
+    Proof.
+      intros ι. destruct_syminstance ι. cbn.
+      iIntros "(%Hpc & _)".
+      iSplitL; auto.
+      iPureIntro.
+      unfold CorrectPC in Hpc.
+      cbn in Hpc.
+      unfold Not_is_perm.
+      apply andb_prop in Hpc; destruct Hpc as [_ Hpc].
+      apply orb_prop in Hpc; destruct Hpc as [H|H];
+        destruct p; auto.
+    Qed.
+
+    Lemma correctPC_subperm_R_sound :
+      ValidLemma lemma_correctPC_subperm_R.
+    Proof.
+      intros ι. destruct_syminstance ι. cbn.
+      iIntros "(%Hpc & _)"; iSplit; auto.
+      iPureIntro.
+      unfold Subperm.
+      unfold CorrectPC in Hpc.
+      cbn in *.
+      apply andb_prop in Hpc; destruct Hpc as [_ Hpc].
+      apply orb_prop in Hpc; destruct Hpc as [H|H];
+        destruct p; auto.
+    Qed.
+
+    Lemma subperm_not_E_sound :
+      ValidLemma lemma_subperm_not_E.
+    Proof.
+      intros ι. destruct_syminstance ι. cbn.
+      iIntros "(%H & %Hsub & _)".
+      iSplitL; auto.
+      iPureIntro.
+      destruct H as [[-> _]|[-> _]];
+        unfold Subperm in Hsub;
+        unfold Not_is_perm; destruct p'; auto.
+    Qed.
+
     Lemma safe_move_cursor_sound :
       ValidLemma lemma_safe_move_cursor.
     Proof.
       intros ι. destruct_syminstance ι. cbn.
-      iIntros "#Hsafe".
-      iSplit; [done|].
-      do 2 rewrite fixpoint_interp1_eq.
+      iIntros "(#Hsafe & (% & _))".
+      iSplit; first done.
+      rewrite ?fixpoint_interp1_eq.
       destruct p; auto.
-      simpl.
-      iModIntro.
-      iModIntro.
-      (* by iIntros. *)
-    Admitted.
+      unfold Not_is_perm, MinCapsSignature.is_perm in H.
+      discriminate.
+    Qed.
 
     Lemma safe_sub_perm_sound :
       ValidLemma lemma_safe_sub_perm.
@@ -624,7 +663,7 @@ Module MinCapsIrisInstanceWithContracts.
       intros ι. destruct_syminstance ι. cbn.
       iIntros "[#Hsafe %Hp]".
       iSplit; [done|].
-      do 2 rewrite fixpoint_interp1_eq.
+      rewrite ?fixpoint_interp1_eq.
       destruct p; destruct p'; trivial;
         destruct Hp; try discriminate.
     Admitted.
@@ -871,8 +910,8 @@ Module MinCapsIrisInstanceWithContracts.
   Proof.
     intros Δ []; eauto using
                        open_ptsreg_sound, close_ptsreg_sound,
-      open_gprs_sound, close_gprs_sound, int_safe_sound,
-      safe_move_cursor_sound, safe_sub_perm_sound,
+      open_gprs_sound, close_gprs_sound, int_safe_sound, correctPC_not_E_sound,
+      correctPC_subperm_R_sound, subperm_not_E_sound, safe_move_cursor_sound, safe_sub_perm_sound,
       safe_within_range_sound, gen_dummy_sound.
   Qed.
 
